WIP: different init state

theories/lang/defs.v
@@ -88,7 +88,7 @@ Definition never_stuck fs e σ :=
   ∀ e' σ', (e, σ) ~{fs}~>* (e', σ') → terminal e' ∨ reducible fs  e' σ'.
 
 Definition init_expr := (Call #["main"] []).
-Definition init_state := (mkState ∅ ∅ [] O O).
+Definition init_state := (mkState ∅ ∅ [O] O 1).
 
 (*=================================== UNUSED =================================*)
 (* Implicit Type (ρ: cfg bor_lang). *)
