theories/sim/local.v
@@ -59,7 +59,9 @@ Inductive _sim_local_body_step (r_f : A) (sim_local_body : SIM)
     (CONT: ∀ r' v_src v_tgt σs' σt'
              (* For any new resource r' that supports the returned values are
                 related w.r.t. (r ⋅ r' ⋅ r_f) *)
-             (VRET: vrel r' (Val v_src) (Val v_tgt)),
+             (VRET: vrel r' (Val v_src) (Val v_tgt))
+             (* Stack unchanged *)
+             (STACK: σt'.(sst) = σt.(sst)),
         ∃ idx', sim_local_body (rc ⋅ r') idx'
                                (fill Ks (Val v_src)) σs'
                                (fill Kt (Val v_tgt)) σt' Φ).
@@ -99,6 +101,27 @@ Proof.
 Qed.
 
 Definition sim_local_body := paco7 _sim_local_body bot7.
+
+Lemma sim_local_body_post_mono r n es σs et σt Φ Φ' :
+  Φ <6= Φ' →
+  sim_local_body r n es σs et σt Φ → sim_local_body r n es σs et σt Φ'.
+Proof.
+  revert r n es σs et σt Φ Φ'. pcofix CIH. intros r0 n es σs et σt Φ Φ' LE SIM.
+  pfold. punfold SIM; [|apply sim_local_body_mono].
+  intros NT r_f WSAT. specialize (SIM NT r_f WSAT) as [NOTS TE SIM].
+  constructor; [done|..].
+  { intros.
+    destruct (TE _ TERM) as (vs' & σs' & r' & idx' & STEP' & WSAT' & HΦ).
+    naive_solver. }
+  inversion SIM.
+  - left. intros.
+    specialize (STEP _ _ STEPT) as (es' & σs' & r' & idx' & STEP' & WSAT' & SIM').
+    exists es', σs', r', idx'. do 2 (split; [done|]).
+    pclearbot. right. eapply CIH; eauto.
+  - econstructor 2; eauto. intros.
+    destruct (CONT _ _ _ σs' σt' VRET STACK) as [idx' SIM'].
+    exists idx'. pclearbot. right. eapply CIH; eauto.
+Qed.
 
 (* Simulating functions:
   - We start after the substitution.
