theories/sim/program.v
@@ -16,16 +16,20 @@ Proof.
   specialize (SIMf ε ebs ebt [] [] init_state init_state) as [idx SIM]; [done..|].
   unfold behave_prog. eapply (adequacy _ _ idx); [apply _| |by apply wf_init_state..].
   eapply sim_local_conf_sim; eauto.
-  econs; eauto; swap 2 4.
+  econs; swap 2 4.
   - econs 1.
   - ss.
   - ss.
-  - eapply (sim_body_step_into_call _ _ _ _ _ [] ebs HCs [] ebs [] ebt HCt [] ebt);
+  - eapply (sim_body_step_over_call _ _ [] [] init_res ε _ _ [] [] ebt ebt [] HCt);
+      [done..|].
+    intros r' vs vt σs' σt' VREL'.
+    admit.
+    (* eapply (sim_body_step_into_call _ _ _ _ _ [] ebs HCs [] ebs [] ebt HCt [] ebt);
       [done..|].
     eapply (sim_body_bind _ _ _ _ [EndCallCtx] [EndCallCtx] (InitCall ebs) (InitCall ebt)).
-    eapply sim_body_post_mono; [|exact SIM].
+    eapply sim_local_body_post_mono; [|exact SIM].
     clear SIM. simpl.
     intros r1 idx1 vs σs vt σt [ESAT (v1 & v2 & Eq1 & Eq2 & VREL)].
-    rewrite Eq1 Eq2. by apply sim_body_end_call.
-  - rewrite right_id. apply wsat_init_state.
+    rewrite Eq1 Eq2. by apply sim_body_end_call. *)
+  - instantiate (1:=ε). rewrite right_id left_id. apply wsat_init_state.
 Qed.
